Fix broken proofs except Open

examples/knot/KnotHeader.v
@@ -152,6 +152,7 @@ Ltac iarg :=
   let INV := constr:("INV") in
   let OPENER := constr:("☃OPENER") in
   let CLOSED := constr:("☃CLOSED") in
+  let TMP := constr:("☃TMP") in
   let ARG := constr:("ARG") in
   eapply (@harg_clo _ PRE INV);
   [eassumption
@@ -159,6 +160,11 @@ Ltac iarg :=
   ];
   let a := fresh "a" in
   intros a; i;
+  let aa := fresh "aa" in
+  mDesEx PRE as aa;
+  mDesAndPureL PRE as TMP PRE;
+  let EQ := fresh "EQ" in
+  mPure TMP as EQ; symmetry in EQ; destruct EQ;
   mDesAndPureR PRE as PRE ARG;
   let EQ := fresh "EQ" in
   mPure ARG as EQ;
@@ -203,10 +209,11 @@ Tactic Notation "icall_weaken" uconstr(ftsp) uconstr(o) uconstr(x) uconstr(a) "w
   let POST := get_fresh_name_tac "POST" in
   let INV := get_fresh_name_tac "INV" in
   let CLOSED := constr:("☃CLOSED") in
+  let TMP := constr:("☃TMP") in
   let OPENER := constr:("☃OPENER") in
   let Hns := select_ihyps Hns in
   let Hns := constr:("☃CLOSED"::"☃OPENER"::Hns) in
-  eapply (@hcall_clo_weaken _ Hns POST INV _ _ ftsp o x _ (inl a));
+  eapply (@hcall_clo_weaken _ Hns POST INV ftsp o x _ (inl a));
   unshelve_goal;
   [|
    eassumption
@@ -218,17 +225,29 @@ Tactic Notation "icall_weaken" uconstr(ftsp) uconstr(o) uconstr(x) uconstr(a) "w
    |
    |on_current ltac:(fun H => try clear H);
     intros ? ? ? ? ? ? [|[?mp_src ?mp_tgt]]; i; simpl;
-    on_current ltac:(fun H => simpl in H);
+    on_current ltac:(fun H => simpl in H)
+    ;
     [mDesSep INV as "☃CLOSED" INV;
+     let ar := fresh "ar" in
+     mDesEx POST as ar;
+     mDesAndPureL POST as TMP POST;
+     let EQ0 := fresh "EQ" in
+     mPure TMP as EQ0; symmetry in EQ0; destruct EQ0;
      mDesAndPureR POST as POST "☃TMP";
      let EQ := fresh in
      mPure "☃TMP" as EQ; inversion EQ;
      mDesSep POST as "☃OPENER" POST
-    |mDesSep INV as "☃CLOSED" INV;
-     mDesAndPureR POST as POST "☃TMP";
-     mDesSep POST as "☃OPENER" POST;
-     mAssertPure False; [iApply (inv_open_unique with "☃OPENER ☃CLOSED")|ss
-    ]]
+    |
+    mDesSep INV as "☃CLOSED" INV;
+    let ar := fresh "ar" in
+    mDesEx POST as ar;
+    mDesAndPureL POST as TMP POST;
+    let EQ0 := fresh "EQ" in
+    mPure TMP as EQ0; symmetry in EQ0; destruct EQ0;
+    mDesAndPureR POST as POST "☃TMP";
+    mDesSep POST as "☃OPENER" POST;
+    mAssertPure False; [iApply (inv_open_unique with "☃OPENER ☃CLOSED")|ss]
+    ]
   ].
 
 Tactic Notation "iret" uconstr(a) :=
@@ -251,7 +270,7 @@ Definition knot_init: (@URA.car knotRA) := knot_frag None.
 Section REC.
   Context `{Σ: GRA.t}.
 
-  Definition mrec_spec (f: nat -> nat) (INV: iProp): ftspec (list val) val :=
+  Definition mrec_spec (f: nat -> nat) (INV: iProp): fspec :=
     mk_simple (X:=nat)
               (fun n => (
                    (fun varg o =>
