examples/delayed_echo/Stack01proof.v
@@ -60,8 +60,8 @@ Section SIMMODSEM.
       unfold ccall. steps. astart 10.
 
       (* load *)
-      acatch. hcall _ (n, 0%Z, a0) _ with "A1"; auto.
-      { iModIntro. iFrame. iSplit; ss. }
+      acatch. hcall _ (n, 0%Z, a1) _ with "A2"; auto.
+      { iModIntro. iFrame. iExists _. iSplit; ss. }
       { splits; ss. eauto with ord_step. }
       mDesAll. clarify. eapply Any.upcast_inj in PURE1. des; clarify.
       steps. erewrite Any.upcast_downcast in *. steps.
@@ -70,72 +70,74 @@ Section SIMMODSEM.
       (* l = [] *)
       { mDesAll. subst.
         (* cmp *)
-        steps. acatch. hcall _ _ _ with "POST"; auto.
+        steps. acatch. hcall _ _ _ with "A"; auto.
         { instantiate (2:=(true,_)). ss. iModIntro.
-          iSplitR; ss. iSplitL; ss. iSplitL; ss. iSplitR; ss.
-          iRight. iRight. iRight. iRight. iPureIntro. ss. }
+          iSplitR; ss. iExists _. iSplitR; ss. iSplitL; ss. iSplitL; ss.
+          iSplitR; ss. iRight. iRight. iRight. iRight. iPureIntro. ss. }
         { split; ss. eauto with ord_step. }
-        mDesAll. clarify. eapply Any.upcast_inj in PURE3. des; clarify.
+        mDesAll. clarify. eapply Any.upcast_inj in PURE2. des; clarify.
         steps. erewrite Any.upcast_downcast in *. steps.
 
         (* ret *)
-        astop. force_l. eexists. steps. hret _; ss.
+        astop. force_l. eexists. steps. hret _; ss. et.
       }
 
       (* l = lhd :: ltl *)
       mDesAll. subst.
-      rewrite points_to_split in ACC. mDesOwn "A2".
+      rewrite points_to_split in ACC. mDesOwn "A3".
 
       (* cmp *)
-      steps. acatch. hcall _ _ _ with "A2"; auto.
+      steps. acatch. hcall _ _ _ with "A3"; auto.
       { instantiate (2:=(false,_)). ss. iModIntro.
-        iSplitR; ss. iSplitL; ss. iSplitL; ss.
+        iSplitR; ss. iExists _. iSplitR; ss. iSplitL; ss. iSplitL; ss.
         iSplitR; ss. iLeft. iExists _, _, _. iSplit; ss. }
       { split; ss. eauto with ord_step. }
-      ss. mDesAll. clarify. eapply Any.upcast_inj in PURE3. des; clarify.
+      ss. mDesAll. clarify. eapply Any.upcast_inj in PURE2. des; clarify.
       steps. erewrite Any.upcast_downcast in *. steps.
 
       (* load *)
-      steps. acatch. hcall _ (a0, 0%Z, v0) _ with "POST1"; auto.
-      { iModIntro. iSplitR; ss. iSplitL; ss. iSplitL; ss. iSplitR; ss. }
+      steps. acatch. hcall _ (_, 0%Z, _) _ with "A3"; auto.
+      { iModIntro. iSplitR; ss. iExists _.
+        iSplitR; ss. iSplitL; ss. iSplitL; ss. iSplitR; ss. }
       { split; ss. eauto with ord_step. }
       ss. mDesAll. clarify. eapply Any.upcast_inj in PURE4. des; clarify.
       steps. erewrite Any.upcast_downcast in *. clarify.
 
       (* load *)
-      steps. acatch. hcall _ (a0, (0+1)%Z, a2) _ with "A"; auto.
-      { iModIntro. iSplitR; ss. iSplitL; ss. iSplitL; ss. iSplitR; ss. }
+      steps. acatch. hcall _ (_, (0+1)%Z, _) _ with "A1"; auto.
+      { iModIntro. iSplitR; ss. iExists _.
+        iSplitR; ss. iSplitL; ss. iSplitL; ss. iSplitR; ss. }
       { split; ss. eauto with ord_step. }
       ss. mDesAll. clarify. eapply Any.upcast_inj in PURE5. des; clarify.
       steps. erewrite Any.upcast_downcast in *. clarify.
 
       (* free *)
-      steps. acatch. hcall _ (a0, 0%Z) _ with "POST2"; auto.
-      { iModIntro. iSplitR; ss. iSplitL; ss. iSplitL; ss.
-        iExists _. iSplitR; ss. }
+      steps. acatch. hcall _ (_, 0%Z) _ with "A3"; auto.
+      { iModIntro. iSplitR; ss. iExists _. iSplitR; ss.
+        iSplitL; ss. iSplitL; ss. iExists _. iSplitR; ss. }
       { split; ss. eauto with ord_step. }
       ss. mDesAll. clarify. des; clarify.
       steps. erewrite Any.upcast_downcast in *. clarify.
 
       (* free *)
-      steps. acatch. hcall _ (a0, (0+1)%Z) _ with "POST1"; auto.
-      { iModIntro. iSplitR; ss. iSplitL; ss. iSplitL; ss.
-        iExists _. iSplitR; ss. }
+      steps. acatch. hcall _ (_, (0+1)%Z) _ with "A1"; auto.
+      { iModIntro. iSplitR; ss. iExists _. iSplitR; ss. iSplitL; ss.
+        iSplitL; ss. iExists _. iSplitR; ss. }
       { split; ss. eauto with ord_step. }
       ss. mDesAll. clarify. des; clarify.
       steps. erewrite Any.upcast_downcast in *. clarify.
 
       (* store *)
-      steps. acatch. hcall _ (n, 0%Z, v0) _ with "POST"; auto.
-      { iModIntro. iSplitR; ss. iSplitL; ss. iSplitL; ss.
-        iExists _. iSplitR; ss. }
+      steps. acatch. hcall _ (_, 0%Z, _) _ with "A"; auto.
+      { iModIntro. iSplitR; ss. iExists _. iSplitR; ss. iSplitL; ss.
+        iSplitL; ss. iExists _. iSplitR; ss. }
       { split; ss. eauto with ord_step. }
       ss. mDesAll. clarify. des; clarify.
       steps. erewrite Any.upcast_downcast in *. clarify.
 
       (* ret *)
       astop. force_l. eexists. steps. hret _; ss.
-      iModIntro. iSplitR; ss. iSplitL; ss. iSplitR; ss.
+      iModIntro. iSplitR; ss. iExists _. iSplitR; ss. iSplitL; ss. iSplitR; ss.
       iExists _. iFrame.
     }
 
@@ -151,16 +153,17 @@ Section SIMMODSEM.
       (* l = [] *)
       { mDesAll. subst.
         (* cmp *)
-        steps. acatch. hcall _ _ _ with "A"; auto.
+        steps. acatch. hcall _ _ _ with "A1"; auto.
         { instantiate (2:=(true,_)). ss. iModIntro.
-          iSplitR; ss. iSplitL; ss. iSplitL; ss. iSplitR; ss.
+          iSplitR; ss. iExists _. iSplitR; ss.
+          iSplitL; ss. iSplitL; ss. iSplitR; ss.
           iRight. iRight. iRight. iRight. iPureIntro. ss. }
         { split; ss. eauto with ord_step. }
         mDesAll. clarify. eapply Any.upcast_inj in PURE1. des; clarify.
         steps. erewrite Any.upcast_downcast in *. steps.
 
         (* ret *)
-        astop. force_l. eexists. steps. hret _; ss.
+        astop. force_l. eexists. steps. hret _; ss. et.
       }
 
       (* l = lhd :: ltl *)
@@ -170,53 +173,55 @@ Section SIMMODSEM.
       (* cmp *)
       steps. acatch. hcall _ _ _ with "A3"; auto.
       { instantiate (2:=(false,_)). ss. iModIntro.
-        iSplitR; ss. iSplitL; ss. iSplitL; ss.
+        iSplitR; ss. iExists _. iSplitR; ss. iSplitL; ss. iSplitL; ss.
         iSplitR; ss. iLeft. iExists _, _, _. iSplit; ss. }
       { split; ss. eauto with ord_step. }
       ss. mDesAll. clarify. eapply Any.upcast_inj in PURE1. des; clarify.
       steps. erewrite Any.upcast_downcast in *. steps.
 
       (* load *)
-      steps. acatch. hcall _ (a2, 0%Z, v) _ with "POST"; auto.
-      { iModIntro. iSplitR; ss. iSplitL; ss. iSplitL; ss. iSplitR; ss. }
+      steps. acatch. hcall _ (_, 0%Z, _) _ with "A3"; auto.
+      { iModIntro. iSplitR; ss. iExists _. iSplitR; ss.
+        iSplitL; ss. iSplitL; ss. iSplitR; ss. }
       { split; ss. eauto with ord_step. }
-      ss. mDesAll. clarify. eapply Any.upcast_inj in PURE3. des; clarify.
+      ss. mDesAll. clarify. eapply Any.upcast_inj in PURE2. des; clarify.
       steps. erewrite Any.upcast_downcast in *. clarify.
 
       (* load *)
-      steps. acatch. hcall _ (a2, (0+1)%Z, a3) _ with "A1"; auto.
-      { iModIntro. iSplitR; ss. iSplitL; ss. iSplitL; ss. iSplitR; ss. }
+      steps. acatch. hcall _ (_, (0+1)%Z, _) _ with "A2"; auto.
+      { iModIntro. iSplitR; ss. iExists _. iSplitR; ss.
+        iSplitL; ss. iSplitL; ss. iSplitR; ss. }
       { split; ss. eauto with ord_step. }
       ss. mDesAll. clarify. eapply Any.upcast_inj in PURE4. des; clarify.
       steps. erewrite Any.upcast_downcast in *. clarify.
 
       (* free *)
-      steps. acatch. hcall _ (a2, 0%Z) _ with "POST1"; auto.
-      { iModIntro. iSplitR; ss. iSplitL; ss. iSplitL; ss.
-        iExists _. iSplitR; ss. }
+      steps. acatch. hcall _ (_, 0%Z) _ with "A3"; auto.
+      { iModIntro. iSplitR; ss. iExists _. iSplitR; ss.
+        iSplitL; ss. iSplitL; ss. iExists _. iSplitR; ss. }
       { split; ss. eauto with ord_step. }
       ss. mDesAll. clarify. des; clarify.
       steps. erewrite Any.upcast_downcast in *. clarify.
 
       (* free *)
-      steps. acatch. hcall _ (a2, (0+1)%Z) _ with "POST"; auto.
-      { iModIntro. iSplitR; ss. iSplitL; ss. iSplitL; ss.
-        iExists _. iSplitR; ss. }
+      steps. acatch. hcall _ (_, (0+1)%Z) _ with "A2"; auto.
+      { iModIntro. iSplitR; ss. iExists _. iSplitR; ss.
+        iSplitL; ss. iSplitL; ss. iExists _. iSplitR; ss. }
       { split; ss. eauto with ord_step. }
       ss. mDesAll. clarify. des; clarify.
       steps. erewrite Any.upcast_downcast in *. clarify.
 
       (* store *)
-      steps. acatch. hcall _ (n, 0%Z, v0) _ with "A"; auto.
-      { iModIntro. iSplitR; ss. iSplitL; ss. iSplitL; ss.
-        iExists _. iSplitR; ss. }
+      steps. acatch. hcall _ (_, 0%Z, _) _ with "A1"; auto.
+      { iModIntro. iSplitR; ss. iExists _. iSplitR; ss.
+        iSplitL; ss. iSplitL; ss. iExists _. iSplitR; ss. }
       { split; ss. eauto with ord_step. }
       ss. mDesAll. clarify. des; clarify.
       steps. erewrite Any.upcast_downcast in *. clarify.
 
       (* ret *)
       astop. force_l. eexists. steps. hret _; ss.
-      iModIntro. iSplitR; ss. iSplitL; ss.
+      iModIntro. iSplitR; ss. iExists _. iSplitR; ss. iSplitL; ss.
       iExists _. iFrame. ss.
     }
 
@@ -233,28 +238,29 @@ Section SIMMODSEM.
       { split; ss. eauto with ord_step. }
       mDesAll. clarify. eapply Any.upcast_inj in PURE1. des; clarify.
       steps. erewrite Any.upcast_downcast in *. steps.
-      rewrite points_to_split in ACC. mDesOwn "A1".
+      rewrite points_to_split in ACC. mDesOwn "A2".
 
       (* store *)
-      steps. acatch. hcall _ (a2, 0%Z, v) _ with "A1"; auto.
-      { rewrite Z.add_0_l. iModIntro. iSplitR; ss. iSplitL; ss.
+      steps. acatch. hcall _ (_, 0%Z, _) _ with "A2"; auto.
+      { rewrite Z.add_0_l. iModIntro. iSplitR; ss.
+        iExists _. iSplitR; ss. iSplitL; ss.
         iSplitL; ss. iExists _. iFrame. et. }
       { split; ss. eauto with ord_step. }
       mDesAll. clarify. erewrite Any.upcast_downcast in *. steps.
 
       (* store *)
-      steps. acatch. hcall _ (a2, (0+1)%Z, a0) _ with "A2"; auto.
-      { iModIntro. iSplitR; ss. iSplitL; ss.
+      steps. acatch. hcall _ (_, (0+1)%Z, _) _ with "A"; auto.
+      { iModIntro. iSplitR; ss. iExists _. iSplitR; ss. iSplitL; ss.
         iSplitL; ss. iExists _. iFrame. et. }
       { split; ss. eauto with ord_step. }
       mDesAll. clarify. erewrite Any.upcast_downcast in *. steps.
 
       (* ret *)
-      mCombine "POST" "POST1".
+      mCombine "A2" "A".
       rewrite <- points_to_split in ACC.
       astop. force_l. eexists. steps. hret _; ss.
-      iModIntro. iSplitR; ss. iSplitL; ss.
-      iExists _. iSplitL; ss. iExists _, _. iSplitR "A"; ss.
+      iModIntro. iSplitR; ss. iExists _. iSplitR; ss. iSplitL; ss.
+      iExists _. iSplitL; ss. iExists _, _. iSplitR "A1"; ss.
       iSplitR; ss.
     }
     Unshelve. all: ss.
