examples/mutsum/MutMain01proof.v
@@ -44,13 +44,12 @@ Section SIMMODSEM.
     unfold mainF, mainBody. harg.
     mDesAll. des; clarify. steps. rewrite Any.upcast_downcast. steps.
     hcall _ _ tt with "*"; ss.
-    { iPureIntro. splits; eauto. instantiate (1:=10). ss. }
+    { iPureIntro. esplits; eauto. instantiate (1:=10). ss. }
     { splits; ss. }
-    mDesAll. des; clarify. eapply Any.upcast_inj in PURE2. des; clarify. steps.
+    mDesAll. des; clarify. eapply Any.upcast_inj in PURE1. des; clarify. steps.
     hret tt; ss.
     (* TODO: change top2 => pure top in SMod.main *)
-    iModIntro. repeat iSplit; ss.
-    iStopProof. red. uipropall.
+    iModIntro. et.
   Qed.
 
 End SIMMODSEM.
